Defining CTX equivalence, and CTX scoping

src/CIU.v
@@ -3,5 +3,29 @@ Import ListNotations.
 
 Definition CIU (e1 e2 : Exp) : Prop :=
   EXPCLOSED e1 /\ EXPCLOSED e2 /\
-  exists v1 v2, (* Vrel v1 v2 /\  <- here n-independent equivalence needed *)
-  (exists clock, eval clock e1 = Res v1) <-> (exists clock, eval clock e2 = Res v2). 
+  forall v1 v2, CIU_equivalent_values v1 v2 ->
+  (exists clock, eval clock e1 = Res v1) <-> (exists clock, eval clock e2 = Res v2).
+
+Definition CIU_open (Γ : list VarFunId) (e1 e2 : Exp) :=
+  forall ξ, subscoped Γ [] ξ ->
+  CIU (subst ξ e1) (subst ξ e2).
+
+Lemma CIU_closed :
+  forall e1 e2,
+  CIU e1 e2 -> EXPCLOSED e1 /\ EXPCLOSED e2.
+Proof.
+  intros. unfold CIU in H. intuition.
+Qed.
+
+
+Lemma Erel_implies_CIU : forall Γ e1 e2,
+  Erel_open Γ e1 e2 ->
+  CIU_open Γ e1 e2.
+Proof.
+  intros. unfold CIU_open, CIU; intros.
+  split. 2: split. 3: assert (EXPCLOSED (subst ξ e1) /\ EXPCLOSED (subst ξ e2)).
+  1-3: eapply Erel_open_closed in H; eauto; apply H.
+  intros. destruct H1. unfold Erel_open, Erel in H. unfold exp_rel in H.
+  split; intros; inversion H3.
+  - unfold CIU_equivalent_values in H2. destruct H2, H2.
+Qed.
